doc/coq/check.sh
@@ -1,0 +1,1 @@
+coqchk -silent -o -R tactics sflib -R simple Simple tactics/*.vo simple/*.vo
